HumanEval43

HumanEvalLean/HumanEval43.lean
@@ -1,5 +1,99 @@
-def pairs_sum_to_zero : Unit :=
-  ()
+import Std.Data.HashSet.Lemmas
+import Std.Tactic.Do
+
+open Std Do
+
+theorem List.exists_mem_iff_exists_getElem (P : α → Prop) (l : List α) :
+    (∃ x ∈ l, P x) ↔ ∃ (i : Nat), ∃ hi, P (l[i]'hi) := by
+  grind [mem_iff_getElem]
+
+structure List.Any₂ (P : α → α → Prop) (l : List α) where
+  not_pairwise : ¬ l.Pairwise (fun x y => ¬P x y)
+
+theorem List.any₂_iff_not_pairwise {P : α → α → Prop} {l : List α} :
+    l.Any₂ P ↔ ¬l.Pairwise (fun x y => ¬P x y) := by
+  grind [List.Any₂]
+
+@[simp, grind]
+theorem not_any₂_nil {P : α → α → Prop} : ¬List.Any₂ P [] := by
+  simp [List.any₂_iff_not_pairwise]
+
+@[simp, grind]
+theorem List.any₂_cons {P : α → α → Prop} {x : α} {xs : List α} :
+    List.Any₂ P (x::xs) ↔ (∃ y ∈ xs, P x y) ∨ List.Any₂ P xs := by
+  grind [List.any₂_iff_not_pairwise]
+
+@[grind]
+theorem List.any₂_append {P : α → α → Prop} {xs ys : List α} :
+    List.Any₂ P (xs ++ ys) ↔ List.Any₂ P xs ∨ List.Any₂ P ys ∨ (∃ x ∈ xs, ∃ y ∈ ys, P x y) := by
+  grind [List.any₂_iff_not_pairwise]
+
+def pairsSumToZero (l : List Int) : Bool :=
+  go l ∅
+where
+  go (m : List Int) (seen : HashSet Int) : Bool :=
+    match m with
+    | [] => false
+    | x::xs => if -x ∈ seen then true else go xs (seen.insert x)
+
+example : pairsSumToZero [1, 3, 5, 0] = false := by native_decide
+example : pairsSumToZero [1, 3, -2, 1] = false := by native_decide
+example : pairsSumToZero [1, 2, 3, 7] = false := by native_decide
+example : pairsSumToZero [2, 4, -5, 3, 5, 7] = true := by native_decide
+example : pairsSumToZero [1] = false := by native_decide
+
+-- `simp` does not solve this!!
+example {x : Int} : -x + x = 0 := by omega
+
+theorem pairsSumToZero_go_iff (l : List Int) (seen : HashSet Int) :
+    pairsSumToZero.go l seen = true ↔
+      l.Any₂ (fun a b => a + b = 0) ∨ ∃ a ∈ seen, ∃ b ∈ l, a + b = 0 := by
+  fun_induction pairsSumToZero.go <;> simp <;> grind
+
+theorem pairsSumToZero_iff (l : List Int) :
+    pairsSumToZero l = true ↔ l.Any₂ (fun a b => a + b = 0) := by
+  simp [pairsSumToZero, pairsSumToZero_go_iff]
+
+def pairsSumToZero' (l : List Int) : Id Bool := do
+  let mut seen : HashSet Int := ∅
+  for x in l do
+    if -x ∈ seen then
+      return true
+    seen := seen.insert x
+  return false
+
+-- Pain: I have no idea what the system wants from me when building an invariant.
+-- What is a PostCond? What does the function I'm returning mean? How are early returns
+-- and things like that represented?
+
+-- Pain: The need to have the `l = z.pref` trick in the loop invariant. If you don't know this
+-- it's hard to make progress. It would be really cool if there was some kind of "interactive"
+-- way to build the loop invariant in multiple steps where I only have to input the
+-- `(∀ x, x ∈ s ↔ x ∈ z.rpref) ∧ ¬ z.pref.Any₂ (fun a b => a + b = 0)` and
+-- `l.Any₂ (fun a b => a + b = 0)` parts and the `o = none/some` and `l = z.pref` gadgets are
+-- added automatically.
+
+-- Pain: `refine` does not play well with `⇓` it seems
+
+-- Pain: mvcgen generated multiple assumptions named `h`, leading to inaccessible names
+-- Pain: mvcgen generally creates inaccessible names
+
+@[simp]
+theorem List.Zipper.pref_mk {l : List α} {rpref suff h} :
+    (List.Zipper.mk rpref suff h : List.Zipper l).pref = rpref.reverse := rfl
+
+set_option mvcgen.warning false
+
+theorem pairsSumToZero'_spec (l : List Int) :
+    ⦃⌜True⌝⦄ pairsSumToZero' l ⦃⇓r => r = true ↔ l.Any₂ (fun a b => a + b = 0)⦄ := by
+  mvcgen [pairsSumToZero']
+
+  case inv =>
+    exact (fun (⟨o, s⟩, z) =>
+      (o = none ∧ (∀ x, x ∈ s ↔ x ∈ z.rpref) ∧ ¬ z.pref.Any₂ (fun a b => a + b = 0)) ∨
+      (o = some true ∧ l.Any₂ (fun a b => a + b = 0) ∧ l = z.pref), ())
+
+  all_goals simp_all [List.any₂_append] <;> grind
 
 /-!
 ## Prompt
@@ -57,3 +151,63 @@ def check(candidate):
 
 ```
 -/
+
+/-! Bonus material -/
+
+theorem List.exists_append (l : List α) (n : Nat) (h : n ≤ l.length) : ∃ xs ys, ys.length = n ∧ l = xs ++ ys :=
+  ⟨l.take (l.length - n), l.drop (l.length - n), by grind, by simp⟩
+
+@[simp]
+theorem Std.HashSet.toList_emptyWithCapacity {α : Type u} [BEq α] [Hashable α]
+    [EquivBEq α] [LawfulHashable α] {n : Nat} :
+    (HashSet.emptyWithCapacity n : HashSet α).toList = [] := by
+  simp [← List.isEmpty_iff]
+
+@[simp]
+theorem Std.HashSet.toList_empty {α : Type u} [BEq α] [Hashable α]
+    [EquivBEq α] [LawfulHashable α] : (∅ : HashSet α).toList = [] := by
+  simp [← List.isEmpty_iff]
+
+theorem List.Any₂.append_left {P : α → α → Prop} (xs : List α) {ys : List α} (h : ys.Any₂ P) : (xs ++ ys).Any₂ P :=
+  List.any₂_append.2 (by simp [h])
+
+theorem List.Any₂.append_right {P : α → α → Prop} {xs : List α} (ys : List α) (h : xs.Any₂ P) : (xs ++ ys).Any₂ P :=
+  List.any₂_append.2 (by simp [h])
+
+theorem List.any₂_append_left_right {P : α → α → Prop} (xs ys : List α) (h : ∃ x ∈ xs, ∃ y ∈ ys, P x y) :
+    (xs ++ ys).Any₂ P :=
+  List.any₂_append.2 (by simp [h])
+
+theorem List.any₂_iff_exists (P : α → α → Prop) (l : List α) :
+    List.Any₂ P l ↔ ∃ xs x ys, l = xs ++ x :: ys ∧ ∃ y ∈ ys, P x y := by
+  constructor
+  · rintro ⟨h⟩
+    induction l with
+    | nil => grind
+    | cons x xs ih =>
+      rw [List.pairwise_cons, Classical.not_and_iff_not_or_not] at h
+      simp only [Classical.not_forall, Classical.not_not] at h
+      rcases h with (⟨y, hy, hxy⟩|h)
+      · exact ⟨[], by grind⟩
+      · grind
+  · grind
+
+theorem List.any₂_iff_exists_getElem (P : α → α → Prop) (l : List α) :
+    List.Any₂ P l ↔ ∃ (i j : Nat), ∃ hi hj, i < j ∧ P (l[i]'hi) (l[j]'hj) := by
+  rw [List.any₂_iff_exists]
+  constructor
+  · rintro ⟨xs, x, ys, ⟨rfl, h⟩⟩
+    obtain ⟨j₀, hj₀, hj₀'⟩ := (List.exists_mem_iff_exists_getElem _ _).1 h
+    exact ⟨xs.length, xs.length + 1 + j₀, by grind⟩
+  · rintro ⟨i, j, hi, hj, hij, h⟩
+    exact ⟨l.take i, l[i], l.drop (i + 1), by simp,
+      (List.exists_mem_iff_exists_getElem _ _).2 ⟨j - i - 1, by grind, by grind⟩⟩
+
+@[simp, grind]
+theorem List.any₂_append_singleton {P : α → α → Prop} {xs : List α} {x : α} :
+    List.Any₂ P (xs ++ [x]) ↔ List.Any₂ P xs ∨ ∃ y ∈ xs, P y x := by
+  grind [List.any₂_iff_not_pairwise]
+
+@[simp, grind]
+theorem not_any₂_singleton {P : α → α → Prop} {x : α} : ¬List.Any₂ P [x] := by
+  simp [List.any₂_iff_not_pairwise]
